\documentclass{revtex4}
\usepackage{amsmath,amssymb}

\input{mynotation}

\begin{document}

\section{Appendix: Modifed Projectors for Discretum Derivatives}

\section{Appendix: Useful Relations}
This just summarizes a collection of useful formulae so I'm not constantly rederiving them.

\subsection{Continuum Projectors}
\begin{equation}
  P_{ij} \equiv \delta_{ij} - \hat{k}_i\hat{k}_j
\end{equation}
which satisfy
\begin{subequations}
\begin{align}
  P_{il}\kzero_l\kzero_j &= \kzero_i\kzero_j - \hat{k}_i\kzero_j\kone \\
  P_{il}\kzero_l\kzero_j\delta_{lj} &= \\
  P_{ij}\kzero_i\kzero_j &= \kzero^2 - \kone^2 \\
  P_{ij}\kzero_i\kzero_j\delta_{ij} &= \, .
\end{align}
\end{subequations}
Combining, we obtain
\begin{subequations}
\begin{align}
  \proj^{(T)}_{ij,lm}\delta_{lm} &= 0 \\
  \proj^{(T)}_{ij,lm}\kzero_l\kzero_m &=  \\
  \proj^{(T)}_{ij,lm}\kzero_l\kzero_m\delta_{lm} &= \, .
\end{align}
\end{subequations}

\subsection{Discrete Factorized Projectors}
Here, let's instead use
\begin{equation}
  Q_{ij} \equiv \delta_{ij} - \frac{\kzero_i\kzero_j}{\kzero^2}
\end{equation}
to contstruct our TT projection operator
\begin{equation}
  \proj^Q_{ij,lm} \equiv Q_{il}Q_{jm} - \frac{1}{2}Q_{ij}Q_{lm}
\end{equation}
We then have
\begin{subequations}
\begin{align}
  \proj^Q_{ij,lm}\delta_{lm} &= 0 \\
  \proj^Q_{ij,lm}\kzero_l\kzero_m &= 0 \\
  \proj^Q_{ij,lm}\kzero_l\kzero_m\delta_{lm} &= \\
  \proj^Q_{ij,lm}C_l\kzero_l\kzero_m &= 
\end{align}
\end{subequations}

\subsection{Trace Squared}
Suppose we have
\begin{equation}
  T_{ij} = C_i\delta_{ij}
\end{equation}
Then we obtain (w/ continuum projectors)
\begin{equation}
  T_{ji}^*\mathcal{O}_{ij,lm}T_{lm} = \sum_i |C_i|^2(1-2\hat{k}_i^2) + \left|\sum_i C_i\hat{k}_i^2\right|^2 - \frac{1}{2}\left|\sum_i C_i(\hat{k}_i^2-1)\right|^2 \, .
\end{equation}
This assumes (can probably relax some of these)
\begin{enumerate}
\item Real valued unit $k$ vectors
\item $\mathcal{O}_{ij,lm}^* = \mathcal{O}_{ij,lm}$
\end{enumerate}
Consider the special case of $C_i = \kzero_i^2$ (i.e.\ $\kzero_i\kzero_j\delta_{ij}$ terms).
Then we obtain
\begin{equation}
  \sum \kzero_m^4(1-2\hat{k}_m^2) + \frac{\ktwo^4}{2} - \frac{\kzero^4}{2} + \kzero^2\ktwo^2 \, .
\end{equation}
Suppose we also have
\begin{equation}
  S_{ij} = A\tilde{k}_i\tilde{k}_j
\end{equation}
We then have the following contraction
\begin{align}
  S_{ij}\mathcal{O}_{ij,lm}T_{lm} &= \kzero_i\kzero_jP_{il}P_{jm}C_l\delta_{lm} - \frac{1}{2}(\kzero^2-\kone^2)\left(\sum_l C_l(1-\hat{k}_l^2)\right) \\
  &= \sum \kzero_l^2C_l - 2\kone\sum C_l\kzero_l\hat{\kone}_l + \kone^2\sum\hat{k}_l^2C_l - \frac{1}{2}(\kzero^2-\kone^2)\left(\sum_l C_l(1-\hat{k}_l^2)\right)
\end{align}

Other useful special cases (in a form with obvious generalization)
\begin{equation}
  \kzero_i\kzero_j\mathcal{O}_{ij,lm}\kzero_l\kzero_m = \left(\kzero_iP_{ij}\kzero_j\right)^2 = \kzero^2-\kone^2
\end{equation}
\begin{equation}
  \kzero_i\kzero_j\mathcal{O}_{ij,lm}\kzero_l\kzero_m\delta_{lm} = 
\end{equation}

\end{document}
